Snapshot

providers/evercrypt/fst/EverCrypt.HMAC.fst
@@ -1,68 +1,56 @@
 (* Agile HMAC *)
 module EverCrypt.HMAC
 
+module S = FStar.Seq
+
 /// Agile specification
 
 open EverCrypt.Helpers
 open FStar.Integers
-open FStar.Seq
 
-let wrap (a:alg) (key: bytes{length key <= maxLength a}): GTot (lbseq (blockLength a))
+noextract inline_for_extraction
+let spec = Spec.Hash.Nist.hash
+
+#set-options "--max_fuel 0 --max_ifuel 0"
+let wrap (a:alg) (key: bytes{S.length key < max_input8 a}): GTot (lbytes (size_block a))
 =
-  let key0 = if length key <= blockLength a then key else spec a key in
-  let paddingLength = blockLength a - length key0 in
-  key0 @| Seq.create paddingLength 0uy
+  let key0 = if S.length key <= size_block a then key else spec a key in
+  let paddingLength = size_block a - S.length key0 in
+  S.append key0 (S.create paddingLength 0uy)
 
-private let wrap_lemma (a:alg) (key: bseq{Seq.length key <= maxLength a}): Lemma
-  (requires length key > blockLength a)
+let wrap_lemma (a:alg) (key: bytes{Seq.length key < max_input8 a}): Lemma
+  (requires S.length key > size_block a)
   (ensures wrap a key == (
     let key0 = spec a key in
-    let paddingLength = blockLength a - length key0 in
-    key0 @| Seq.create paddingLength 0uy)) = ()
+    let paddingLength = size_block a - S.length key0 in
+    S.append key0 (S.create paddingLength 0uy))) = ()
 
 // better than Integer's [^^] to tame polymorphism in the proof?
 inline_for_extraction
 let xor8 (x y: uint8_t): uint8_t = x ^^ y
 
-let xor (x: uint8_t) (v: bseq): GTot (lbseq (length v)) =
+let xor (x: uint8_t) (v: bytes): GTot (lbytes (S.length v)) =
   Spec.Loops.seq_map (xor8 x) v
 
-let rec xor_lemma (x: uint8_t) (v: bseq) : Lemma (requires True)
-  (ensures (xor x v == Spec.Loops.seq_map2 xor8 (create (length v) x) v))
-  (decreases (length v)) =
-  let l = length v in
+#push-options "--max_fuel 1"
+let rec xor_lemma (x: uint8_t) (v: bytes) : Lemma (requires True)
+  (ensures (xor x v == Spec.Loops.seq_map2 xor8 (S.create (S.length v) x) v))
+  (decreases (S.length v)) =
+  let l = S.length v in
   if l = 0 then () else (
-    let xs  = create l x in
-    let xs' = create (l-1) x in
-    lemma_eq_intro (tail xs) xs';
-    xor_lemma x (tail v))
-(*
-    assert(// by induction
-      xor (tail v) y == Spec.Loops.seq_map2 xor8 (tail v) ys');
-    assert(// by definition
-      Spec.Loops.seq_map (fun x -> xor8 x y) v ==
-      cons
-        (xor8 (head v) y)
-        (Spec.Loops.seq_map (fun x -> xor8 x y) (tail v)));
-    assert(// by definition
-      xor v y ==
-      cons
-        (xor8 (head v) y)
-        (xor (tail v) y));
-    assert(// by definition
-      Spec.Loops.seq_map2 xor8 v ys ==
-      cons
-        (xor8 (head v) (head ys))
-        (Spec.Loops.seq_map2 xor8 (tail v) (tail ys)));
-*)
+    let xs  = S.create l x in
+    let xs' = S.create (l-1) x in
+    S.lemma_eq_intro (S.tail xs) xs';
+    xor_lemma x (S.tail v))
+#pop-options
 
 let hmac a key data =
-  assert(tagLength a + blockLength a <= maxLength a); // avoidable?
   let k = wrap a key in
-  let h1 = spec a (xor 0x36uy k @| data) in
-  let h2 = spec a (xor 0x5cuy k @| h1) in
+  let h1 = spec a S.(xor 0x36uy k @| data) in
+  assert_norm (pow2 32 < pow2 61);
+  assert_norm (pow2 32 < pow2 125);
+  let h2 = spec a S.(xor 0x5cuy k @| h1) in
   h2
-
 
 
 /// Agile implementation
@@ -76,37 +64,47 @@ module ST = FStar.HyperStack.ST
 
 // we rely on the output being zero-initialized for the correctness of padding
 
-#set-options "--max_fuel 0"
+#set-options "--max_fuel 0 --max_ifuel 0 --z3rlimit 50"
 
 inline_for_extraction
 val wrap_key:
   a: ha ->
-  output: uint8_pl (blockLength a) ->
-  key: uint8_p {length key <= maxLength a /\ disjoint output key} ->
+  output: uint8_pl (size_block a) ->
+  key: uint8_p {length key < max_input8 a /\ disjoint output key} ->
   len: UInt32.t {v len = length key} ->
   Stack unit
     (requires fun h0 ->
       live h0 output /\ live h0 key /\
-      as_seq h0 output == Seq.create (blockLength a) 0uy)
+      as_seq h0 output == Seq.create (size_block a) 0uy)
     (ensures fun h0 _ h1 ->
       live h1 output /\ live h1 key /\ live h0 output /\ live h0 key /\
-      as_seq h0 output == Seq.create (blockLength a) 0uy /\
+      as_seq h0 output == Seq.create (size_block a) 0uy /\
       modifies (loc_buffer output) h0 h1 /\
       as_seq h1 output = wrap a (as_seq h0 key) )
 
 inline_for_extraction
+let block_len a = Hacl.Hash.Definitions.size_block_ul a
+
+inline_for_extraction
+let tag_len a = Hacl.Hash.Definitions.size_hash_ul a
+
+
+// let key0 = if S.length key <= size_block a then key else spec a key in
+// let paddingLength = size_block a - S.length key0 in
+// S.append key0 (S.create paddingLength 0uy)
+inline_for_extraction
 let wrap_key a output key len =
   //[@inline_let] //18-08-02 does *not* prevents unused-but-set-variable warning in C
-  let i = if len <= blockLen a then len else tagLen a in
+  let i = if len <= block_len a then len else tag_len a in
   let nkey = sub output 0ul i in
   let h0 = ST.get () in
-  if len <= blockLen a then
+  if len <= block_len a then
     blit key 0ul nkey 0ul len
   else
     Hash.hash a nkey key len;
   let h1 = ST.get () in (
-    let pad = sub output i (blockLen a - i) in
-    Seq.lemma_eq_intro (as_seq h0 pad) (Seq.create (blockLength a - v i) 0uy);
+    let pad = sub output i (block_len a - i) in
+    Seq.lemma_eq_intro (as_seq h0 pad) (Seq.create (size_block a - v i) 0uy);
     Seq.lemma_split (as_seq h1 output) (v i)
   )
 
@@ -117,10 +115,10 @@ inline_for_extraction
 val part1:
   a: alg -> 
   acc: state a ->
-  s2: uint8_pl (blockLength a) ->
+  s2: uint8_pl (size_block a) ->
   data: uint8_p {
-    length data + blockLength a  < pow2 32 /\ (*required by 32-bit length for update_last *)
-    // length data + blockLength a <= maxLength a /\ (*always true*)
+    length data + size_block a  < pow2 32 /\ (*required by 32-bit length for update_last *)
+    // length data + size_block a <= max_input8 a /\ (*always true*)
     disjoint data s2} ->
   len: UInt32.t {length data = v len} ->
   ST unit
@@ -136,8 +134,8 @@ val part1:
       footprint acc h1 == footprint acc h0 /\ //18-08-02 avoidable? this footprint is constant!
       modifies (loc_union (footprint acc h0) (loc_buffer s2)) h0 h1 /\
       (
-      let hash0 = Seq.slice (as_seq h1 s2) 0 (tagLength a) in
-      length data + blockLength a <= maxLength a /\ (*always true, required by spec below*)
+      let hash0 = Seq.slice (as_seq h1 s2) 0 (size_hash a) in
+      length data + size_block a <= max_input8 a /\ (*always true, required by spec below*)
       hash0 == spec a (Seq.append (as_seq h0 s2) (as_seq h0 data))))
 
 #reset-options "--max_fuel 0 --z3rlimit 1000" // without hints
@@ -145,8 +143,8 @@ val part1:
 // we use auxiliary functions only for clarity and proof modularity
 inline_for_extraction
 let part1 a (acc: state a) key data len =
-  assert_norm(pow2 32 + blockLength a <= maxLength a);
-  let ll = len % blockLen a in
+  assert_norm(pow2 32 + size_block a <= max_input8 a);
+  let ll = len % block_len a in
   let lb = len - ll in
   let blocks = sub data 0ul lb in
   let last = offset data lb in
@@ -166,19 +164,19 @@ let part1 a (acc: state a) key data len =
     (Ghost.hide (as_seq h0 key))
     acc blocks lb;
   let h2 = ST.get() in
-  assert_norm(blockLength a + v len <= maxLength a);
+  assert_norm(size_block a + v len <= max_input8 a);
   Hash.update_last 
     #(Ghost.hide a)
     (Ghost.hide (Seq.append (as_seq h0 key) (as_seq h2 blocks)))
-    acc last (blockLen a + len);
+    acc last (block_len a + len);
   let h3 = ST.get() in
   // assert(LowStar.Buffer.live h3 key);
-  let tag = sub key 0ul (tagLen a) in (* Salvage memory *)
+  let tag = sub key 0ul (tag_len a) in (* Salvage memory *)
   Hash.finish #(Ghost.hide a) acc tag;
   let h4 = ST.get() in
   (
     modifies_trans (footprint acc h0) h0 h3 (loc_buffer key) h4; // should this implicitly trigger?
-    let p = blockLength a in
+    let p = size_block a in
     let key1 = as_seq h1 key in
     let blocks1 = as_seq h1 blocks in
     let acc1 = repr acc h1 in
@@ -212,9 +210,9 @@ inline_for_extraction
 val part2:
   a: alg -> 
   acc: state a ->
-  mac: uint8_pl (tagLength a) ->
-  opad: uint8_pl (blockLength a) ->
-  tag: uint8_pl (tagLength a) ->
+  mac: uint8_pl (size_hash a) ->
+  opad: uint8_pl (size_block a) ->
+  tag: uint8_pl (size_hash a) ->
   ST unit
     (requires fun h0 ->
       invariant acc h0 /\
@@ -229,13 +227,13 @@ val part2:
       invariant acc h1 /\ footprint acc h1 == footprint acc h0 /\
       modifies (loc_union (footprint acc h0) (loc_buffer mac)) h0 h1 /\
       ( let payload = Seq.append (as_seq h0 opad) (as_seq h0 tag) in
-        Seq.length payload <= maxLength a /\
+        Seq.length payload <= max_input8 a /\
         as_seq h1 mac = spec a payload))
 
 inline_for_extraction
 let part2 a acc mac opad tag =
-  let totLen = blockLen a + tagLen a in
-  assert_norm(v totLen <= maxLength a);
+  let totLen = block_len a + tag_len a in
+  assert_norm(v totLen <= max_input8 a);
   let h0 = ST.get() in
   //assume(LowStar.Modifies.(loc_disjoint (footprint acc h0) (loc_buffer opad)));
   Hash.init #(Ghost.hide a) acc;
@@ -261,23 +259,23 @@ let part2 a acc mac opad tag =
     lemma_compress (acc0 #a) v1;
     assert(acc1 == hash0 v1);
     let tag1 = as_seq h1 tag in
-    let suffix1 = suffix a (blockLength a + tagLength a) in
+    let suffix1 = suffix a (size_block a + size_hash a) in
     let acc2 = repr acc h2 in
     lemma_hash2 (acc0 #a) v1 (tag1 @| suffix1);
     Seq.append_assoc v1 tag1 suffix1;
     assert(acc2 == hash0 ((v1 @| tag1) @| suffix1));
     assert(extract acc2 = spec a (v1 @| tag1)))
 
-// similar spec as hmac with keylen = blockLen a
+// similar spec as hmac with keylen = block_len a
 inline_for_extraction
 val hmac_core:
   a: alg -> 
   acc: state a ->
-  tag: uint8_pl (tagLength a) ->
-  key: uint8_pl (blockLength a) {disjoint key tag} ->
+  tag: uint8_pl (size_hash a) ->
+  key: uint8_pl (size_block a) {disjoint key tag} ->
   data: uint8_p{
-    length data + blockLength a < pow2 32 /\ (*required for 32-bit allocation*)
-    // length data + blockLength a <= maxLength a /\ (*always true*)
+    length data + size_block a < pow2 32 /\ (*required for 32-bit allocation*)
+    // length data + size_block a <= max_input8 a /\ (*always true*)
     disjoint data key } ->
   datalen: UInt32.t {v datalen = length data} ->
   ST unit
@@ -296,9 +294,9 @@ val hmac_core:
     ( let k = as_seq h0 key in
       let k1 = xor 0x36uy k in
       let k2 = xor 0x5cuy k in
-      length data + blockLength a <= maxLength a /\ ( (*always true*)
+      length data + size_block a <= max_input8 a /\ ( (*always true*)
       let v1 = spec a (k1 @| as_seq h0 data) in
-      Seq.length (k2 @| v1) <= maxLength a /\
+      Seq.length (k2 @| v1) <= max_input8 a /\
       as_seq h1 tag == spec a (k2 @| v1))))
 
 inline_for_extraction
@@ -327,14 +325,14 @@ let hmac_core a acc tag key data len =
   fresh_frame_modifies h00 h01; //18-08-02 a trigger would be nice!
   Hash.frame_invariant loc_none acc h00 h01;
   // assert(invariant acc h01);
-  let ipad = alloca 0x36uy (blockLen a) in
+  let ipad = alloca 0x36uy (block_len a) in
   let h02 = ST.get() in
   //  assert (loc_in (footprint acc h01) h01);
   // TR: now works thanks to Hash.invariant_loc_in_footprint
   fresh_is_disjoint (loc_buffer ipad) (footprint acc h01)  h01 h02;
-  let opad = alloca 0x5cuy (blockLen a) in
-  xor_bytes_inplace ipad key (blockLen a);
-  xor_bytes_inplace opad key (blockLen a);
+  let opad = alloca 0x5cuy (block_len a) in
+  xor_bytes_inplace ipad key (block_len a);
+  xor_bytes_inplace opad key (block_len a);
   let h0 = ST.get() in
   modifies_address_liveness_insensitive_unused_in h01 h0;
   // assert(loc_in (footprint acc h0) h0);
@@ -344,19 +342,19 @@ let hmac_core a acc tag key data len =
   frame_invariant (loc_union (loc_buffer ipad) (loc_buffer opad)) acc h01 h0;
   part1 a acc ipad data len;
   let h1 = ST.get() in
-  let inner = sub ipad 0ul (tagLen a) in (* salvage memory *)
+  let inner = sub ipad 0ul (tag_len a) in (* salvage memory *)
   part2 a acc tag opad inner;
   let h2 = ST.get() in
   pop_frame ();
   (
     let h3 = ST.get() in
     let k = as_seq h0 key in
-    let k1: lbseq (blockLength a) = xor 0x36uy k in
-    let k2: lbseq (blockLength a) = xor 0x5cuy k in
+    let k1: lbytes (size_block a) = xor 0x36uy k in
+    let k2: lbytes (size_block a) = xor 0x5cuy k in
     let vdata = as_seq h0 data in
-    let v1: lbseq (tagLength a) = as_seq h1 inner in
-    assert_norm(blockLength a + tagLength a <= maxLength a);
-    assert(Seq.length (k2 @| v1) <= maxLength a);
+    let v1: lbytes (size_hash a) = as_seq h1 inner in
+    assert_norm(size_block a + size_hash a <= max_input8 a);
+    assert(Seq.length (k2 @| v1) <= max_input8 a);
     let v2 = as_seq h2 tag in
     xor_lemma 0x36uy k;
     xor_lemma 0x5cuy k;
@@ -392,9 +390,9 @@ inline_for_extraction
 let compute a mac key keylen data datalen =
   let h00 = ST.get() in
   push_frame ();
-  assert_norm(pow2 32 + blockLength a <= maxLength a);
-  assert(length data + blockLength a <= maxLength a);
-  let keyblock = alloca 0x00uy (blockLen a) in
+  assert_norm(pow2 32 + size_block a <= max_input8 a);
+  assert(length data + size_block a <= max_input8 a);
+  let keyblock = alloca 0x00uy (block_len a) in
   let acc = Hash.create a in
   let h0 = ST.get() in
   wrap_key a keyblock key keylen;
@@ -420,8 +418,8 @@ let compute a mac key keylen data datalen =
 
 let compute a mac key keylen data datalen =
   push_frame ();
-  assert_norm(pow2 32 <= maxLength a);
-  let keyblock = Buffer.create 0x00uy (blockLen a) in
+  assert_norm(pow2 32 <= max_input8 a);
+  let keyblock = Buffer.create 0x00uy (block_len a) in
   wrap_key a keyblock key keylen;
   ( match a with
   | SHA256 ->
@@ -447,8 +445,8 @@ let compute a mac key keylen data datalen =
 
 let compute a mac key keylen data datalen =
   push_frame ();
-  let keyblock = Buffer.create 0x00uy (blockLen a) in
-  assert_norm(pow2 32 <= maxLength a);
+  let keyblock = Buffer.create 0x00uy (block_len a) in
+  assert_norm(pow2 32 <= max_input8 a);
   wrap_key a keyblock key keylen;
   let acc =
     match a with
